reorganize

Communication_Topology_Analysis.thy
@@ -2,6 +2,116 @@ theory Communication_Topology_Analysis
   imports Main Syntax Semantics Abstract_Value_Flow_Analysis
 begin
 
+  
+definition send_sites :: "state_pool \<Rightarrow> chan \<Rightarrow> control_path set" where
+  "send_sites \<E> ch = {\<pi>. \<exists> x x\<^sub>e e \<kappa> \<rho> x\<^sub>c x\<^sub>m \<rho>\<^sub>e. 
+    \<E> \<pi> = Some (<<LET x = SYNC x\<^sub>e in e, \<rho>, \<kappa>>>) \<and> 
+    \<rho> x\<^sub>e = Some \<lbrace>Send_Evt x\<^sub>c x\<^sub>m, \<rho>\<^sub>e\<rbrace> \<and> 
+    \<rho>\<^sub>e x\<^sub>c = Some \<lbrace>ch\<rbrace>
+  }"
+
+definition recv_sites :: "state_pool \<Rightarrow> chan \<Rightarrow> control_path set" where
+  "recv_sites \<E> ch = {\<pi>. \<exists> x x\<^sub>e e \<kappa> \<rho> x\<^sub>c \<rho>\<^sub>e. 
+    \<E> \<pi> = Some (<<LET x = SYNC x\<^sub>e in e, \<rho>, \<kappa>>>) \<and> 
+    \<rho> x\<^sub>e = Some \<lbrace>Recv_Evt x\<^sub>c, \<rho>\<^sub>e\<rbrace> \<and> 
+    \<rho>\<^sub>e x\<^sub>c = Some \<lbrace>ch\<rbrace>
+  }"
+
+definition single_side' :: "(state_pool \<Rightarrow> chan \<Rightarrow> control_path set) \<Rightarrow> state_pool \<Rightarrow> var \<Rightarrow> bool" where
+  "single_side' sites_of \<E> x \<longleftrightarrow> (\<forall> \<pi> \<pi>\<^sub>1 \<pi>\<^sub>2 .
+    \<pi>\<^sub>1 \<in> sites_of \<E> (Ch \<pi> x) \<longrightarrow>
+    \<pi>\<^sub>2 \<in> sites_of \<E> (Ch \<pi> x) \<longrightarrow>
+    (prefix \<pi>\<^sub>1 \<pi>\<^sub>2 \<or> prefix \<pi>\<^sub>2 \<pi>\<^sub>1) 
+  )"  
+
+definition single_side :: "(state_pool \<Rightarrow> chan \<Rightarrow> control_path set) \<Rightarrow> exp \<Rightarrow> var \<Rightarrow> bool" where
+  "single_side sites_of e x \<equiv> (\<forall> \<E>'. 
+    [[] \<mapsto> <<e, empty, []>>] \<rightarrow>* \<E>' \<longrightarrow>
+    single_side' sites_of \<E>' x
+  )"  
+
+definition one_shot' :: "state_pool \<Rightarrow> var \<Rightarrow> bool" where
+  "one_shot' \<E> x \<longleftrightarrow> (\<forall> \<pi> . \<E> (\<pi>;;x) \<noteq> None \<longrightarrow>
+    card (send_sites \<E> (Ch \<pi> x)) \<le> 1
+  )"
+
+definition one_shot :: "exp \<Rightarrow> var \<Rightarrow> bool" where
+  "one_shot e x \<longleftrightarrow> (\<forall> \<E>' .
+    [[] \<mapsto> <<e, empty, []>>] \<rightarrow>* \<E>' \<longrightarrow>
+    one_shot' \<E>' x
+  )"
+
+
+definition single_receiver' :: "state_pool \<Rightarrow> var \<Rightarrow> bool" where 
+  "single_receiver' = single_side' recv_sites"
+
+definition single_receiver :: "exp \<Rightarrow> var \<Rightarrow> bool" where 
+  "single_receiver = single_side recv_sites"
+  
+
+definition single_sender' :: "state_pool \<Rightarrow> var \<Rightarrow> bool" where 
+  "single_sender' = single_side' recv_sites"
+
+definition single_sender :: "exp \<Rightarrow> var \<Rightarrow> bool" where 
+  "single_sender = single_side send_sites"
+
+definition point_to_point' :: "state_pool \<Rightarrow> var \<Rightarrow> bool" where
+  "point_to_point' \<E> x \<longleftrightarrow> single_sender' \<E> x \<and> single_receiver' \<E> x"
+  
+definition point_to_point :: "exp \<Rightarrow> var \<Rightarrow> bool" where
+  "point_to_point e x \<longleftrightarrow> single_sender e x \<and> single_receiver e x"
+  
+definition fan_out' :: "state_pool \<Rightarrow> var \<Rightarrow> bool" where
+  "fan_out' \<E> x \<longleftrightarrow> single_sender' \<E> x \<and> \<not> single_receiver' \<E> x "
+
+definition fan_out :: "exp \<Rightarrow> var \<Rightarrow> bool" where
+  "fan_out e x \<longleftrightarrow> single_sender e x \<and> \<not> single_receiver e x "
+  
+definition fan_in' :: "state_pool \<Rightarrow> var \<Rightarrow> bool" where
+  "fan_in' \<E> x \<longleftrightarrow> \<not> single_sender' \<E> x \<and> single_receiver' \<E> x "
+
+definition fan_in :: "exp \<Rightarrow> var \<Rightarrow> bool" where
+  "fan_in e x \<longleftrightarrow> \<not> single_sender e x \<and> single_receiver e x "
+
+datatype topo = OneShot | OneToOne | FanOut | FanIn | Any
+
+type_synonym topo_pair = "var \<times> topo"
+
+type_synonym topo_env = "var \<Rightarrow> topo"
+
+definition env_to_topo_env :: "state_pool \<Rightarrow> topo_env" ("\<langle>\<langle>_\<rangle>\<rangle>" [0]61) where
+  "\<langle>\<langle>\<E>\<rangle>\<rangle> = (\<lambda> x . 
+    (if one_shot' \<E> x then OneShot
+    else (if point_to_point' \<E> x then OneToOne
+    else (if fan_out' \<E> x then FanOut
+    else (if fan_in' \<E> x then FanOut
+    else Any))))
+  )"
+
+definition exp_to_topo_env :: "exp \<Rightarrow> topo_env" ("\<langle>\<langle>\<langle>_\<rangle>\<rangle>\<rangle>" [0]61) where
+  "\<langle>\<langle>\<langle>e\<rangle>\<rangle>\<rangle> = (\<lambda> x . 
+    (if one_shot e x then OneShot
+    else (if point_to_point e x then OneToOne
+    else (if fan_out e x then FanOut
+    else (if fan_in e x then FanOut
+    else Any))))
+  )"
+
+inductive precision_order :: "topo \<Rightarrow> topo \<Rightarrow> bool" (infix "\<preceq>" 55) where  
+  Edge1 : "OneShot \<preceq> OneToOne" | 
+  Edge2 : "OneToOne \<preceq> FanOut" |
+  Edge3 : "OneToOne \<preceq> FanIn" |
+  Edge4 : "FanOut \<preceq> Any" |
+  Edge5 : "FanIn \<preceq> Any" |
+  Refl : "t \<preceq> t" |
+  Trans : "\<lbrakk> a \<preceq> b ; b \<preceq> c \<rbrakk> \<Longrightarrow> a \<preceq> c"
+
+definition topo_env_prevision :: "topo_env \<Rightarrow> topo_env \<Rightarrow> bool" (infix "\<sqsubseteq>\<^sub>t" 55) where
+  "\<A> \<sqsubseteq>\<^sub>t \<A>' \<equiv> (\<forall> x . \<A> x \<preceq> \<A>' x)"
+
+
+
+
 type_synonym abstract_path = "(var + unit) list"
 
 
@@ -70,101 +180,75 @@ inductive subexp :: "exp \<Rightarrow> exp \<Rightarrow> bool" where
   Refl: "subexp e e" |
   Step: "subexp e' e \<Longrightarrow> subexp e' (LET _ = _ in e)"
 
-definition send_sites :: "var \<Rightarrow> exp \<Rightarrow> var set" where
-  "send_sites c e = {x . \<exists> y e' z \<V> \<C>. 
+definition abstract_send_sites :: "var \<Rightarrow> exp \<Rightarrow> var set" where
+  "abstract_send_sites c e = {x . \<exists> y e' z \<V> \<C>. 
     subexp (LET x = SYNC y in e') e \<and> 
     (\<V>, \<C>) \<Turnstile> e \<and> 
     ^Send_Evt c z \<in> \<V> y
   }"
 
-definition recv_sites :: "var \<Rightarrow> exp \<Rightarrow> var set" where
-  "recv_sites c e = {x . \<exists> y e' \<V> \<C>. 
+definition abstract_recv_sites :: "var \<Rightarrow> exp \<Rightarrow> var set" where
+  "abstract_recv_sites c e = {x . \<exists> y e' \<V> \<C>. 
     subexp (LET x = SYNC y in e') e \<and> 
     (\<V>, \<C>) \<Turnstile> e \<and> 
     ^Recv_Evt c \<in> \<V> y
   }"
 
 
-definition paths :: "var set \<Rightarrow> exp \<Rightarrow> abstract_path set" where 
-  "paths sites e = {path @ [Inl x] | path x . 
+definition abstract_paths :: "var set \<Rightarrow> exp \<Rightarrow> abstract_path set" where 
+  "abstract_paths sites e = {path @ [Inl x] | path x . 
     (x \<in> sites) \<and>  path_in_exp (path @ [Inl x]) e
   }" 
 
-definition processes :: "var set \<Rightarrow> exp \<Rightarrow> abstract_path set" where 
-  "processes sites e = {\<pi> \<in> paths sites e .
-    (\<exists> \<pi>' . (\<pi> @ [Inr ()] @ \<pi>') \<in> paths sites e) \<or>
-    (\<forall> \<pi>' . (\<pi> @ \<pi>') \<notin> paths sites e)
+definition abstract_processes :: "var set \<Rightarrow> exp \<Rightarrow> abstract_path set" where 
+  "abstract_processes sites e = {\<pi> \<in> abstract_paths sites e .
+    (\<exists> \<pi>' . (\<pi> @ [Inr ()] @ \<pi>') \<in> abstract_paths sites e) \<or>
+    (\<forall> \<pi>' . (\<pi> @ \<pi>') \<notin> abstract_paths sites e)
   }" 
 
-definition send_paths where 
-  "send_paths c e = paths (send_sites c e) e"
+definition abstract_send_paths where 
+  "abstract_send_paths c e = abstract_paths (abstract_send_sites c e) e"
 
-definition recv_paths where 
-  "recv_paths c e = paths (recv_sites c e) e"
+definition abstract_recv_paths where 
+  "abstract_recv_paths c e = abstract_paths (abstract_recv_sites c e) e"
 
-definition send_processes where 
-  "send_processes c e = processes (send_sites c e) e"
+definition abstract_send_processes where 
+  "abstract_send_processes c e = abstract_processes (abstract_send_sites c e) e"
 
-definition recv_processes where 
-  "recv_processes c e = processes (recv_sites c e) e"
+definition abstract_recv_processes where 
+  "abstract_recv_processes c e = abstract_processes (abstract_recv_sites c e) e"
 
 definition one_max :: "abstract_path set \<Rightarrow> bool"  where
   "one_max \<T> \<equiv>  (\<nexists> p . p \<in> \<T>) \<or> (\<exists>! p . p \<in> \<T>)"
 
 
-datatype topo = OneShot | OneToOne | FanOut | FanIn | Any
-
-type_synonym topo_pair = "var \<times> topo"
-
 inductive communication_topology' :: "topo_pair \<Rightarrow> exp \<Rightarrow> bool" (infix "\<parallel>\<bind>" 55) where
   OneShot: "
-    one_max (send_paths c e) \<Longrightarrow> 
+    one_max (abstract_send_paths c e) \<Longrightarrow> 
     (c, OneShot) \<parallel>\<bind> e
   " | 
   OneToOne: "
     \<lbrakk> 
-      one_max (send_processes c e) ;
-      one_max (recv_processes c e) 
+      one_max (abstract_send_processes c e) ;
+      one_max (abstract_recv_processes c e) 
     \<rbrakk> \<Longrightarrow> 
     (c, OneToOne) \<parallel>\<bind> e
   " | 
 
   FanOut: "
-    one_max (send_processes c e) \<Longrightarrow> 
+    one_max (abstract_send_processes c e) \<Longrightarrow> 
     (c, FanOut) \<parallel>\<bind> e
   " | 
 
   FanIn: "
-    one_max (recv_processes c e) \<Longrightarrow> 
+    one_max (abstract_recv_processes c e) \<Longrightarrow> 
     (c, FanIn) \<parallel>\<bind> e
   " | 
 
   Any: "(c, Any) \<parallel>\<bind> e"
 
 
-type_synonym topo_env = "var \<Rightarrow> topo"
-
 definition communication_topology :: "topo_env \<Rightarrow> exp \<Rightarrow> bool" (infix "\<bind>" 55) where 
   "\<A> \<bind> e \<longleftrightarrow> (\<forall> x . (x, \<A> x) \<parallel>\<bind> e)"
 
-definition env_to_topo_env :: "state_pool \<Rightarrow> topo_env" ("\<langle>\<langle>_\<rangle>\<rangle>" [0]61) where
-  "\<langle>\<langle>\<E>\<rangle>\<rangle> = (\<lambda> x . 
-    (if one_shot' \<E> x then OneShot
-    else (if point_to_point' \<E> x then OneToOne
-    else (if fan_out' \<E> x then FanOut
-    else (if fan_in' \<E> x then FanOut
-    else Any))))
-  )"
-
-inductive precision_order :: "topo \<Rightarrow> topo \<Rightarrow> bool" (infix "\<preceq>" 55) where  
-  Edge1 : "OneShot \<preceq> OneToOne" | 
-  Edge2 : "OneToOne \<preceq> FanOut" |
-  Edge3 : "OneToOne \<preceq> FanIn" |
-  Edge4 : "FanOut \<preceq> Any" |
-  Edge5 : "FanIn \<preceq> Any" |
-  Refl : "t \<preceq> t" |
-  Trans : "\<lbrakk> a \<preceq> b ; b \<preceq> c \<rbrakk> \<Longrightarrow> a \<preceq> c"
-
-definition topo_env_prevision :: "topo_env \<Rightarrow> topo_env \<Rightarrow> bool" (infix "\<sqsubseteq>\<^sub>t" 55) where
-  "\<A> \<sqsubseteq>\<^sub>t \<A>' \<equiv> (\<forall> x . \<A> x \<preceq> \<A>' x)"
 end
